Cleanup

formal-verification/FormalVerification/DeletionCircuit.lean
@@ -4,6 +4,7 @@ import ProvenZk.Merkle
 import ProvenZk.Ext.Vector
 
 import FormalVerification
+import FormalVerification.Utils
 import FormalVerification.SemanticEquivalence
 
 open SemaphoreMTB (F Order)
@@ -15,40 +16,6 @@ open SemaphoreMTB renaming DeletionRound_30_30 → gDeletionRound
 open SemaphoreMTB renaming DeletionProof_4_4_30_4_4_30 → gDeletionProof
 
 set_option pp.coercions false
-
-------------------- MISC
-
-def is_index_in_range {n : Nat} (D : Nat) (a : ZMod n) : Prop :=
-  a.val < 2^D
-
-def are_indices_in_range {d n : Nat} (D : Nat) (a : Vector (ZMod n) d) : Prop :=
-  List.foldr (fun x r => (is_index_in_range D x) ∧ r) True a.toList
-
-theorem are_indices_in_range_cons {d n : Nat} (D : Nat) (a : ZMod n) (vec : Vector (ZMod n) d) :
-  are_indices_in_range D (a ::ᵥ vec) ↔ is_index_in_range D a ∧ are_indices_in_range D vec := by
-  unfold are_indices_in_range
-  conv => lhs; unfold List.foldr; simp
-
-theorem are_indices_in_range_split {d n : Nat} (D : Nat) (a : Vector (ZMod n) (d+1)) :
-  are_indices_in_range D a ↔ is_index_in_range D a.head ∧ are_indices_in_range D a.tail := by
-  rw [<-are_indices_in_range_cons]
-  simp
-
-lemma head_index_in_range {b : Nat} (D : Nat) (Index : Vector (ZMod n) (b+1)) (xs_small : are_indices_in_range D Index) :
-  is_index_in_range D (Vector.head Index) := by
-  rw [are_indices_in_range_split] at xs_small
-  cases xs_small
-  rename_i x xs
-  simp [x]
-
-lemma tail_index_in_range {b : Nat} (D : Nat) (Index : Vector (ZMod n) (b+1)) (xs_small : are_indices_in_range D Index) :
-  are_indices_in_range D (Vector.tail Index) := by
-  rw [are_indices_in_range_split] at xs_small
-  cases xs_small
-  rename_i x xs
-  simp [xs]
-
-------------------
 
 def TreeDelete [Fact (perfect_hash poseidon₂)]
   (Tree : MerkleTree F poseidon₂ D) (Skip : Bit) (Path : Vector F D) : MerkleTree F poseidon₂ D :=
