formal-verification/FormalVerification/InsertionCircuit.lean
@@ -4,6 +4,7 @@ import ProvenZk.Merkle
 import ProvenZk.Ext.Vector
 
 import FormalVerification
+import FormalVerification.Utils
 import FormalVerification.SemanticEquivalence
 
 open SemaphoreMTB (F Order)
@@ -16,215 +17,591 @@ open SemaphoreMTB renaming InsertionProof_4_30_4_4_30 → gInsertionProof
 
 set_option pp.coercions false
 
-def TreeInsert [Fact (perfect_hash poseidon₂)] (Tree : MerkleTree F poseidon₂ D) (Index Item : F) (Proof : Vector F D) (k : F → Prop): Prop :=
-  MerkleTree.item_at_nat Tree Index.val = some 0 ∧
-  MerkleTree.proof_at_nat Tree Index.val = some Proof.reverse ∧
-  ∃postTree, MerkleTree.set_at_nat Tree Index.val Item = some postTree ∧
-  k postTree.root
+------------ MISC
 
-theorem insertion_round_uncps [Fact (perfect_hash poseidon₂)] (Tree : MerkleTree F poseidon₂ D) (Index Item : F) (Proof : Vector F D) (k : F → Prop):
-  insertion_round_prep Index Item Tree.root Proof k ↔
-  TreeInsert Tree Index Item Proof k := by
-  unfold insertion_round_prep
+lemma proof_of_set
+  {F d}
+  (H : Hash F 2)
+  [Fact (perfect_hash H)]
+  (Tree : MerkleTree F H d)
+  (ix : Vector Dir d)
+  (item : F):
+  (MerkleTree.proof (MerkleTree.set Tree ix item) ix) = MerkleTree.proof Tree ix := by
+  induction d with
+  | zero =>
+    simp [MerkleTree.set, MerkleTree.proof]
+  | succ d ih =>
+    cases Tree
+    simp [MerkleTree.set, MerkleTree.proof, MerkleTree.tree_for]
+    split
+    . rename_i hdir
+      have : Dir.swap (Dir.swap (Vector.head ix)) = Dir.right := by
+        rw [hdir]
+        simp [Dir.swap]
+      have : Vector.head ix = Dir.right := by
+        rw [<-this]
+        simp [Dir.swap]
+        cases ix.head
+        . simp
+        . simp
+      rw [this]
+      simp [MerkleTree.set, MerkleTree.left, MerkleTree.right]
+      simp [Vector.vector_eq_cons]
+      rw [ih]
+    . rename_i hdir
+      have : Dir.swap (Dir.swap (Vector.head ix)) = Dir.left := by
+        rw [hdir]
+        simp [Dir.swap]
+      have : Vector.head ix = Dir.left := by
+        rw [<-this]
+        simp [Dir.swap]
+        cases ix.head
+        . simp
+        . simp
+      rw [this]
+      simp [MerkleTree.set, MerkleTree.left, MerkleTree.right]
+      simp [Vector.vector_eq_cons]
+      rw [ih]
+
+def tree_item_at_fin {F: Type} {H: Hash F 2} (Tree : MerkleTree F H d) (i : Fin (2^d)): F :=
+  MerkleTree.item_at Tree (Dir.fin_to_dir_vec i).reverse
+
+def tree_proof_at_fin {F: Type} {H: Hash F 2} (Tree : MerkleTree F H d) (i : Fin (2^d)): Vector F d :=
+  MerkleTree.proof Tree (Dir.fin_to_dir_vec i).reverse
+
+def tree_set_at_fin {F: Type} {H: Hash F 2} (Tree : MerkleTree F H d) (i : Fin (2^d)) (Item : F): MerkleTree F H d :=
+  MerkleTree.set Tree (Dir.fin_to_dir_vec i).reverse Item
+
+------------
+
+def TreeInsert [Fact (perfect_hash poseidon₂)]
+  (Tree : MerkleTree F poseidon₂ D) (Path : Vector F D) (Item : F) : MerkleTree F poseidon₂ D :=
+  MerkleTree.set Tree (Dir.create_dir_vec Path).reverse Item
+
+theorem insertion_round_item_validation [Fact (perfect_hash poseidon₂)]
+  (Tree : MerkleTree F poseidon₂ D) (Path : Vector F D) (Proof : Vector F D) (k : F → Prop) :
+  insertion_round Path Item Tree.root Proof k → (0:F) = MerkleTree.item_at Tree (Dir.create_dir_vec Path).reverse := by
+  intro ⟨H, _⟩
+  rw [MerkleTree.recover_tail_equals_recover_reverse] at H
+  exact Eq.symm (MerkleTree.proof_ceritfies_item _ _ _ _ H)
+
+theorem insertion_round_proof_validation [Fact (perfect_hash poseidon₂)]
+  (Tree : MerkleTree F poseidon₂ D) (Path : Vector F D) (Item: F) (Proof : Vector F D) (k : F → Prop) :
+  insertion_round Path Item Tree.root Proof k → Proof = (MerkleTree.proof Tree (Dir.create_dir_vec Path).reverse).reverse := by
+  intro ⟨H, _⟩
+  rw [MerkleTree.recover_tail_equals_recover_reverse] at H
+  apply Eq.symm
+  rw [Vector.vector_reverse_eq]
+  exact MerkleTree.recover_proof_reversible H
+
+def TreeInsertZeroVector [Fact (perfect_hash poseidon₂)]
+  (Tree : MerkleTree F poseidon₂ D) (Path : Vector F D) : Prop :=
+  MerkleTree.item_at Tree (Dir.create_dir_vec Path).reverse = (0:F)
+
+def TreeInsertZeroZMod [Fact (perfect_hash poseidon₂)]
+  (Tree : MerkleTree F poseidon₂ D) (Index : F) : Prop :=
+  tree_item_at_fin Tree Index.val = (0:F)
+
+-- def TreeInsertZero_equivalence [Fact (perfect_hash poseidon₂)]
+--   (Tree : MerkleTree F poseidon₂ D) (Index : F) (ix_small : is_index_in_range D Index) :
+--   let path := fin_to_bits_le ⟨Index.val, ix_small⟩
+--   TreeInsertZeroZMod Tree Index = TreeInsertZeroVector Tree (Vector.map Bit.toZMod path) := by
+--   sorry
+
+theorem insertion_round_uncps [Fact (perfect_hash poseidon₂)]
+  (Tree : MerkleTree F poseidon₂ D) (Path : Vector F D) (Item : F) (hzero : TreeInsertZeroVector Tree Path) (k : F → Prop) :
+  (let newTree := (MerkleTree.set Tree (Dir.create_dir_vec Path).reverse Item)
+  let item := MerkleTree.item_at newTree (Dir.create_dir_vec Path).reverse
+  let proof := (MerkleTree.proof newTree (Dir.create_dir_vec Path).reverse).reverse
+  insertion_round Path item Tree.root proof k) ↔
+  k (TreeInsert Tree Path Item).root := by
+  simp
   unfold insertion_round
   unfold TreeInsert
+  simp [MerkleTree.recover_tail_equals_recover_reverse]
+  simp [MerkleTree.recover_proof_is_root]
+  intro
+  rw [<-hzero]
+  rw [proof_of_set]
+  simp [MerkleTree.recover_proof_is_root]
+
+theorem insertion_round_prep_index_validation
+  (Root Index Item : F) (Proof : Vector F D) (k : F → Prop) :
+  insertion_round_prep Index Item Root Proof k → is_index_in_range D Index := by
+  unfold insertion_round_prep
+  intro ⟨out, prop, is_bin, _⟩
+  rw [recover_binary_zmod_bit is_bin] at prop
+  rw [←prop]
+  simp [is_index_in_range]
+  rw [binary_nat_zmod_equiv_mod_p]
+  apply Nat.lt_of_le_of_lt
+  apply Nat.mod_le
+  apply binary_nat_lt
+
+theorem insertion_round_prep_zero [Fact (perfect_hash poseidon₂)]
+  (Tree : MerkleTree F poseidon₂ D) (Index : F) (Item : F) (ix_small : is_index_in_range D Index) (k : F → Prop) :
+  let newTree := tree_set_at_fin Tree Index.val Item
+  let item := tree_item_at_fin newTree Index.val
+  let proof := tree_proof_at_fin newTree Index.val
+  insertion_round_prep Index item Tree.root proof.reverse k → TreeInsertZeroZMod Tree Index := by
+  simp
+  unfold insertion_round_prep
+  rintro ⟨ixbin, _⟩
+  casesm* (_ ∧ _)
+  rename_i h
+  simp [TreeInsertZeroZMod]
+  simp [insertion_round] at h
+  casesm* (_ ∧ _)
+  rename_i hrecov hixbin h _
+  simp [tree_item_at_fin]
+  simp [MerkleTree.recover_tail_equals_recover_reverse] at h
+  rw [tree_proof_at_fin, tree_set_at_fin] at h
+  rw [proof_of_set] at h
+  apply MerkleTree.proof_ceritfies_item
+  . rw [ZMod.cast_eq_val]
+    rw [Dir.recover_binary_zmod'_to_dir (w := ixbin)]
+    . rw [h]
+    . simp [is_index_in_range] at ix_small
+      simp [ix_small]
+    . simp [Order]
+    . simp [hixbin]
+    . simp [hrecov]
+
+def TreeInsertPrep [Fact (perfect_hash poseidon₂)]
+  (Tree : MerkleTree F poseidon₂ D) (Index : F) (Item : F) (ix_small : is_index_in_range D Index) : MerkleTree F poseidon₂ D :=
+  let path := fin_to_bits_le ⟨Index.val, ix_small⟩
+  TreeInsert Tree (Vector.map Bit.toZMod path) Item
+
+theorem insertion_round_prep_uncps [Fact (perfect_hash poseidon₂)]
+  (Tree : MerkleTree F poseidon₂ D) (Index : F) (Item : F) (ix_small : is_index_in_range D Index) (hzero : TreeInsertZeroZMod Tree Index) (k : F → Prop) :
+  (let newTree := tree_set_at_fin Tree Index.val Item
+  let item := tree_item_at_fin newTree Index.val
+  let proof := tree_proof_at_fin newTree Index.val
+  insertion_round_prep Index item Tree.root proof.reverse k) ↔
+  k (TreeInsertPrep Tree Index Item ix_small).root := by
+  simp
+  -- intro hzero
+  unfold insertion_round_prep
   apply Iff.intro
   . rintro ⟨ixbin, _⟩
     casesm* (_ ∧ _)
-    have : nat_to_bits_le D Index.val = some (vector_zmod_to_bit ixbin) := by
-      apply recover_binary_zmod'_to_bits_le
+    rename_i h
+    rw [tree_item_at_fin, tree_proof_at_fin, tree_set_at_fin] at h
+    rw [ZMod.cast_eq_val] at h
+    rw [Dir.recover_binary_zmod'_to_dir (w := ixbin)] at h
+    . unfold TreeInsertPrep
+      rw [insertion_round_uncps] at h
+      rw [fin_to_bits_le_to_recover_binary_zmod' (v := Index) (w := ixbin)]
       . simp
-      . assumption
-      . rename_i h _ _ _; simp[h]
-    unfold MerkleTree.item_at_nat
-    unfold MerkleTree.proof_at_nat
-    unfold MerkleTree.set_at_nat
-    unfold Dir.nat_to_dir_vec
-    rw [this]
-    simp [←Dir.create_dir_vec_bit]
-    rename_i h₀ h₁ h₂ h₃
-    refine ⟨?_, ⟨?_, ?_⟩⟩
-    . apply MerkleTree.proof_ceritfies_item (proof := Proof.reverse)
-      rw [←MerkleTree.recover_tail_reverse_equals_recover]
-      simp [h₂]
-    . apply MerkleTree.recover_proof_reversible
-      rw [←MerkleTree.recover_tail_reverse_equals_recover (item := (0:F))]
-      simp [h₂]
-    . rw [←MerkleTree.proof_insert_invariant (proof := Proof.reverse) (old := 0)]
-      . rw [←MerkleTree.recover_tail_reverse_equals_recover]
-        simp [h₃]
-      . rw [←MerkleTree.recover_tail_reverse_equals_recover]
-        simp [h₂]
-  . rintro ⟨hitem, ⟨hproof, ⟨ftree, ⟨hftree, hresult⟩⟩⟩⟩
-    simp [MerkleTree.item_at_nat, Dir.nat_to_dir_vec] at hitem
-    rcases hitem with ⟨bits, ⟨hbits, hitem_at⟩⟩
-    simp [MerkleTree.proof_at_nat, Dir.nat_to_dir_vec] at hproof
-    rcases hproof with ⟨bits', ⟨hbits', hproof_at⟩⟩
-    simp [hbits] at hbits'
-    simp [hbits'] at *
-    simp [MerkleTree.set_at_nat, Dir.nat_to_dir_vec] at hftree
-    rcases hftree with ⟨bits'', ⟨hbits'', hftree_at⟩⟩
-    simp [hbits''] at hbits
-    rw [←Vector.vector_reverse_eq] at hproof_at
-    simp [hbits] at *
-    simp [<-hproof_at]
-    let t : Vector F D := (Vector.map Bit.toZMod bits')
-    refine ⟨t, ?_⟩
-    refine ⟨?_, ⟨?_, ⟨?_, ?_⟩⟩⟩
-    . apply recover_binary_of_to_bits
-      simp [hbits'']
-    . apply vector_binary_of_bit_to_zmod
-    . rw [MerkleTree.recover_tail_equals_recover_reverse, Dir.create_dir_vec_bit, zmod_to_bit_coe, ←hitem_at]
-      simp [MerkleTree.recover_proof_is_root]
-    . rw [<-hftree_at] at hresult
-      rw [MerkleTree.recover_tail_equals_recover_reverse, Dir.create_dir_vec_bit, zmod_to_bit_coe]
-      rw [MerkleTree.proof_insert_invariant _]
-      . apply hresult
-      . exact 0
-      . rw [← hitem_at]
-        simp [MerkleTree.recover_proof_is_root]
-
-theorem before_insertion_all_items_zero_loop
-  [Fact (perfect_hash poseidon₂)]
-  {Tree: MerkleTree F poseidon₂ D}
-  {StartIndex B: Nat}
-  {ixBound: StartIndex + B < Order}
-  {IdComms: Vector F B} {MerkleProofs: Vector (Vector F D) B} {k: F -> Prop}:
-  insertion_rounds ↑StartIndex Tree.root IdComms MerkleProofs k →
-  (∀ i ∈ [StartIndex:StartIndex + B], MerkleTree.item_at_nat Tree i = some 0) := by
-  induction B generalizing StartIndex Tree with
-  | zero =>
-    intro _ i range
-    rcases range with ⟨lo, hi⟩
-    have := Nat.ne_of_lt (Nat.lt_of_le_of_lt lo hi)
-    contradiction
-  | succ B ih =>
-    intro hp i range
-    rcases range with ⟨lo, hi⟩; simp at lo hi
-    have hStartIndexCast : ZMod.val (StartIndex : F) = StartIndex := by
-      apply ZMod.val_cast_of_lt
-      linarith
-    cases lo with
-    | refl =>
-      simp [insertion_rounds, InsertionRound_uncps, insertion_round_uncps, TreeInsert, hStartIndexCast] at hp
-      cases hp
-      rename_i l r
-      simp [l]
-    | @step StartIndex' h =>
-      have : (StartIndex : F) + 1 = ((StartIndex + 1 : Nat) : F) := by
-        simp [Fin.ext]
-      rw [insertion_rounds, InsertionRound_uncps, insertion_round_uncps, TreeInsert, this] at hp
-      rcases hp with ⟨_, ⟨_, ⟨postTree, ⟨hinsert, hnext⟩⟩⟩⟩
-      rw [←MerkleTree.item_at_nat_invariant hinsert]
-      apply ih hnext StartIndex'.succ
-      . apply And.intro
-        . simp_arith; simp [Nat.le] at h; simp [h]
-        . simp; linarith
-      . linarith
-      . rw [hStartIndexCast]
-        apply Nat.ne_of_lt
-        simp_arith; simp [Nat.le] at h; simp [h]
-
-def insertion_circuit [Fact (perfect_hash poseidon₂)] (Tree : MerkleTree F poseidon₂ D) (StartIndex : F) (IdComms: Vector F b) (MerkleProofs: Vector (Vector F D) b) (k : F → Prop): Prop :=
-  match b with
-  | Nat.zero => k Tree.root
-  | Nat.succ _ => MerkleTree.item_at_nat Tree StartIndex.val = some 0 ∧
-                  MerkleTree.proof_at_nat Tree StartIndex.val = some MerkleProofs.head.reverse ∧
-                  ∃postTree, MerkleTree.set_at_nat Tree StartIndex.val IdComms.head = some postTree ∧
-                  insertion_circuit postTree StartIndex.succ IdComms.tail MerkleProofs.tail k
-
-theorem insertion_is_set
-  [Fact (perfect_hash poseidon₂)]
-  {Tree: MerkleTree F poseidon₂ D}
-  (StartIndex: Nat) (IdComms: Vector F b) (MerkleProofs: Vector (Vector F D) b) (PostRoot : F)
-  {ixBound: StartIndex + b < Order}:
-  (InsertionLoop ↑StartIndex Tree.root IdComms MerkleProofs fun newRoot => PostRoot = newRoot) ↔
-  (insertion_circuit Tree ↑StartIndex IdComms MerkleProofs fun newRoot => PostRoot = newRoot) := by
-  apply Iff.intro
-  . induction b generalizing StartIndex Tree with
-    | zero =>
-      simp [InsertionLoop, insertion_circuit]
-    | succ _ ih =>
-      simp only [InsertionLoop, insertion_circuit, insertion_round_prep, insertion_round]
-      rintro ⟨ixbin, _⟩
-      casesm* (_ ∧ _)
-      have : nat_to_bits_le D (↑StartIndex:F).val = some (vector_zmod_to_bit ixbin) := by
-        apply recover_binary_zmod'_to_bits_le
-        . simp
+        rw [vector_zmod_to_bit_to_zmod]
+        . simp [h]
         . assumption
-        . rename_i h _ _ _; simp[h]
-      rename_i h₀ h₁ h₂ h₃
-      unfold MerkleTree.item_at_nat
-      unfold MerkleTree.proof_at_nat
-      unfold MerkleTree.set_at_nat
-      unfold Dir.nat_to_dir_vec
-      rw [this]
-      simp [←Dir.create_dir_vec_bit]
-      refine ⟨?_, ⟨?_, ?_⟩⟩
-      . apply MerkleTree.proof_ceritfies_item (proof := MerkleProofs.head.reverse)
-        rw [<-MerkleTree.recover_tail_equals_recover_reverse]
-        simp [h₂]
-      . apply MerkleTree.recover_proof_reversible (Item := (0:F))
-        rw [<-MerkleTree.recover_tail_equals_recover_reverse]
-        simp [h₂]
-      . have this : MerkleTree.recover_tail poseidon₂ (Dir.create_dir_vec ixbin) (Vector.head MerkleProofs) (Vector.head IdComms) = (MerkleTree.set Tree (Vector.reverse (Dir.create_dir_vec ixbin)) (Vector.head IdComms)).root := by
-          simp [MerkleTree.recover_tail_equals_recover_reverse]
-          apply MerkleTree.proof_insert_invariant (old := (0:F)) (new := IdComms.head)
-          rw [<-MerkleTree.recover_tail_equals_recover_reverse]
-          simp [h₂]
-        simp [this] at h₃
-        have : ((Nat.cast (Fin.val (Nat.cast StartIndex:F))) + (1:F)) = Nat.cast (StartIndex + 1) := by
-          simp [Nat.cast, NatCast.natCast]
-          simp [Order]
-          rw [<-ZMod.val_nat_cast, ZMod.val_cast_of_lt]
-          simp [Order] at ixBound
-          linarith [ixBound]
-        rw [this]
-        apply ih
-        linarith only [ixBound]
-        simp [h₃]
-  . induction b generalizing StartIndex Tree with
+      . simp [ix_small]
+      . assumption
+      . assumption
+      . assumption
+      . rw [TreeInsertZeroZMod, tree_item_at_fin] at hzero
+        rw [TreeInsertZeroVector]
+        rw [Dir.recover_binary_zmod'_to_dir (w := ixbin)] at hzero
+        . simp [hzero]
+        . rw [is_index_in_range] at ix_small
+          simp [ix_small]
+        . simp [Order]
+        . assumption
+        . assumption
+    . simp [is_index_in_range] at ix_small
+      simp [ix_small]
+    . simp [Order]
+    . assumption
+    . assumption
+  . intro h
+    simp [TreeInsertPrep] at h
+    let t : Vector F D := Vector.map Bit.toZMod (fin_to_bits_le ⟨Index.val, ix_small⟩)
+    refine ⟨t, ?_⟩
+    rw [tree_item_at_fin, tree_proof_at_fin, tree_set_at_fin]
+    rw [ZMod.cast_eq_val]
+    rw [Dir.recover_binary_zmod'_to_dir (w := t)]
+    rw [insertion_round_uncps]
+    simp
+    refine ⟨?_, ?_, ?_⟩
+    . rw [recover_binary_of_to_bits]
+      rw [fin_to_bits_le]
+      split
+      . assumption
+      . contradiction
+    . simp [vector_binary_of_bit_to_zmod]
+    . simp [h]
+    . rw [TreeInsertZeroZMod, tree_item_at_fin] at hzero
+      rw [TreeInsertZeroVector]
+      rw [Dir.recover_binary_zmod'_to_dir (w := t)] at hzero
+      . simp [hzero]
+      . rw [is_index_in_range] at ix_small
+        simp [ix_small]
+      . simp [Order]
+      . simp [vector_binary_of_bit_to_zmod]
+      . rw [recover_binary_of_to_bits]
+        simp [fin_to_bits_le]
+        split
+        . assumption
+        . contradiction
+    . rw [is_index_in_range] at ix_small
+      simp [ix_small]
+    . simp [Order]
+    . simp [vector_binary_of_bit_to_zmod]
+    . rw [recover_binary_of_to_bits]
+      simp [fin_to_bits_le]
+      split
+      . assumption
+      . contradiction
+
+-- theorem deletion_round_set_zero [Fact (perfect_hash poseidon₂)]
+--   (Tree : MerkleTree F poseidon₂ D) (Index Item : F) (ix_small : is_index_in_range D Index) :
+--   TreeInsertPrep Tree Index Item ix_small = t →
+--   TreeInsertZero Tree Index ix_small := by
+--   intro htree
+--   unfold TreeInsertPrep at htree
+--   unfold TreeInsert at htree
+--   simp [TreeInsertZero]
+--   apply MerkleTree.set_implies_item_at (t₁ := Tree)
+--   sorry
+
+def TreeInsertCircuit [Fact (perfect_hash poseidon₂)] {b : Nat}
+  (InitialTree : MerkleTree F poseidon₂ D) (StartIndex : Nat) (IdComms: Vector F b) (xs_small : is_index_in_range_nat D (StartIndex + b)) (k : MerkleTree F poseidon₂ D → Prop) : Prop :=
+  match b with
+  | Nat.zero => k InitialTree
+  | Nat.succ i =>
+    ∃newTree, TreeInsertPrep InitialTree StartIndex IdComms.head (by
+    apply is_index_in_range_nat_sum (a := StartIndex) (b := Nat.succ i)
+    . simp [D]
+    . simp [xs_small]) = newTree ∧
+    TreeInsertCircuit newTree (StartIndex+1) IdComms.tail (by
+    simp
+    have : StartIndex + Nat.succ i = StartIndex + 1 + i := by
+      simp [<-Nat.add_one, add_assoc]
+      simp [add_comm]
+    rw [<-this]
+    simp [xs_small]) k
+
+-- TreeInsertCircuitZero
+
+-- before_insertion_all_zeroes
+
+def InsertionLoopTree [Fact (perfect_hash poseidon₂)] {b : Nat}
+  (Tree : MerkleTree F poseidon₂ D) (StartIndex : Nat) (IdComms: Vector F b) (xs_small : is_index_in_range_nat D (StartIndex + b)) (k : MerkleTree F poseidon₂ D → Prop) : Prop :=
+  match b with
+  | Nat.zero => k Tree
+  | Nat.succ i =>
+    let newTree := tree_set_at_fin Tree (StartIndex:F).val IdComms.head
+    let item := tree_item_at_fin newTree (StartIndex:F).val
+    let proof := tree_proof_at_fin newTree (StartIndex:F).val
+    ∃t : MerkleTree F poseidon₂ D,
+    insertion_round_prep StartIndex item Tree.root proof.reverse (fun nextRoot => t.root = nextRoot) ∧
+      InsertionLoopTree t (StartIndex+1) IdComms.tail (by
+    simp
+    have : StartIndex + Nat.succ i = StartIndex + 1 + i := by
+      simp [<-Nat.add_one, add_assoc]
+      simp [add_comm]
+    rw [<-this]
+    simp [xs_small]) k
+
+def InsertionLoopZero [Fact (perfect_hash poseidon₂)] {b : Nat}
+  (Tree : MerkleTree F poseidon₂ D) (StartIndex : Nat) (IdComms: Vector F b) (xs_small : is_index_in_range_nat D (StartIndex + b)) : Prop :=
+  match b with
+  | Nat.zero => True
+  | Nat.succ i =>
+    let t := TreeInsertPrep Tree StartIndex IdComms.head (by
+    apply is_index_in_range_nat_sum (a := StartIndex) (b := Nat.succ i)
+    . simp [D]
+    . simp [xs_small])
+
+    tree_item_at_fin Tree (StartIndex:F).val = (0:F) ∧
+    InsertionLoopZero t (StartIndex+1) IdComms.tail (by
+    simp
+    have : StartIndex + Nat.succ i = StartIndex + 1 + i := by
+      simp [<-Nat.add_one, add_assoc]
+      simp [add_comm]
+    rw [<-this]
+    simp [xs_small])
+
+theorem insertion_loop_uncps [Fact (perfect_hash poseidon₂)] {b : Nat}
+  (Tree : MerkleTree F poseidon₂ D) (StartIndex : Nat) (IdComms: Vector F b) (xs_small : is_index_in_range_nat D (StartIndex + b)) (hzero : InsertionLoopZero Tree StartIndex IdComms xs_small) (k : MerkleTree F poseidon₂ D → Prop) :
+  (TreeInsertCircuit Tree StartIndex IdComms xs_small k ↔
+  InsertionLoopTree Tree StartIndex IdComms xs_small k) := by
+  induction b generalizing Tree StartIndex with
+  | zero =>
+    simp [TreeInsertCircuit, InsertionLoopTree]
+  | succ _ ih =>
+    simp only [TreeInsertCircuit, InsertionLoopTree]
+    simp [InsertionLoopZero] at hzero
+    rcases hzero with ⟨hzero, hnext⟩
+    apply Iff.intro
+    . rintro ⟨tree, htree, hroot⟩
+      refine ⟨tree, ?_, ?_⟩
+      rw [insertion_round_prep_uncps]
+      . rw [MerkleTree.eq_root_eq_tree]
+        apply Eq.symm
+        . simp [htree]
+        . rename_i i
+          apply is_index_in_range_nat_sum (a := StartIndex) (b := Nat.succ i)
+          . simp [D]
+          . simp [xs_small]
+      . rw [TreeInsertZeroZMod]
+        simp [hzero]
+      . rw [<-ih]
+        . simp [hroot]
+        . rw [<-htree]
+          simp [hnext]
+    . rintro ⟨tree, htree, hroot⟩
+      refine ⟨tree, ?_⟩
+      rw [insertion_round_prep_uncps] at htree
+      refine ⟨?_, ?_⟩
+      . rw [<-MerkleTree.eq_root_eq_tree]
+        simp [htree]
+      . rw [ih]
+        . simp [hroot]
+        . rename_i i _
+          let t₁ := tree
+          let t₂ := TreeInsertPrep Tree (StartIndex) (IdComms.head) (by
+          apply is_index_in_range_nat_sum (a := StartIndex) (b := Nat.succ i)
+          . simp [D]
+          . simp [xs_small])
+          rw [MerkleTree.eq_root_eq_tree (t₁ := t₁) (t₂ := t₂)] at htree
+          simp at htree
+          rw [htree]
+          simp [hnext]
+      . rw [TreeInsertZeroZMod]
+        simp [hzero]
+
+def list_of_items_insert [Fact (perfect_hash poseidon₂)]
+  (Tree : MerkleTree F poseidon₂ D) (StartIndex : Nat) (IdComms: Vector F b) (xs_small : is_index_in_range_nat D (StartIndex + b)) : Vector F b :=
+  match b with
+  | Nat.zero => Vector.nil
+  | Nat.succ i =>
+    let t := (tree_set_at_fin Tree (StartIndex:F).val IdComms.head)
+
+    let item_at := tree_item_at_fin t (StartIndex:F).val
+    let tail := list_of_items_insert t (StartIndex+1) IdComms.tail (by
+    simp
+    have : StartIndex + Nat.succ i = StartIndex + 1 + i := by
+      simp [<-Nat.add_one, add_assoc]
+      simp [add_comm]
+    rw [<-this]
+    simp [xs_small])
+    item_at ::ᵥ tail
+
+def list_of_proofs_insert {b : Nat} [Fact (perfect_hash poseidon₂)]
+  (Tree : MerkleTree F poseidon₂ D) (StartIndex : Nat) (IdComms: Vector F b) (xs_small : is_index_in_range_nat D (StartIndex + b)) : Vector (Vector F D) b :=
+  match b with
+  | Nat.zero => Vector.nil
+  | Nat.succ i =>
+    let t := (tree_set_at_fin Tree (StartIndex:F).val IdComms.head)
+
+    let proof := (tree_proof_at_fin t (StartIndex:F).val).reverse
+    let tail := list_of_proofs_insert t (StartIndex+1) IdComms.tail (by
+    simp
+    have : StartIndex + Nat.succ i = StartIndex + 1 + i := by
+      simp [<-Nat.add_one, add_assoc]
+      simp [add_comm]
+    rw [<-this]
+    simp [xs_small])
+
+    proof ::ᵥ tail
+
+@[simp]
+lemma list_of_items_insert_tail {b : Nat} [Fact (perfect_hash poseidon₂)]
+  (Tree : MerkleTree F poseidon₂ D) (StartIndex : Nat) (IdComms: Vector F (b+1)) (xs_small : is_index_in_range_nat D (StartIndex + b + 1)) :
+  Vector.tail (list_of_items_insert Tree StartIndex IdComms xs_small) =
+  let t := TreeInsertPrep Tree (StartIndex:F) IdComms.head (by
+  apply is_index_in_range_nat_sum (a := StartIndex) (b := b + 1)
+  . simp [D]
+  . rw [<-add_assoc]
+    simp [xs_small])
+  list_of_items_insert t (StartIndex+1) IdComms.tail (by
+  simp
+  have : StartIndex + 1 + b = StartIndex + b + 1 := by
+    simp [<-Nat.add_one, add_assoc]
+    simp [add_comm]
+  rw [this]
+  simp [xs_small]) := by
+  simp
+  simp [list_of_items_insert]
+  simp [tree_set_at_fin]
+  simp [TreeInsertPrep]
+  simp [TreeInsert]
+  rw [<-Dir.recover_binary_zmod'_to_dir]
+  . tauto
+  . rw [is_index_in_range_nat] at xs_small
+    rw [ZMod.val_cast_of_lt]
+    . linarith
+    . simp [D] at xs_small
+      simp [Order]
+      linarith
+  . simp [Order, D]
+  . simp [vector_binary_of_bit_to_zmod]
+  . rw [recover_binary_of_to_bits]
+    simp [fin_to_bits_le]
+    split
+    . tauto
+    . contradiction
+
+@[simp]
+lemma list_of_proofs_insert_tail {b : Nat} [Fact (perfect_hash poseidon₂)]
+  (Tree : MerkleTree F poseidon₂ D) (StartIndex : Nat) (IdComms: Vector F (b+1)) (xs_small : is_index_in_range_nat D (StartIndex + b + 1)) :
+  Vector.tail (list_of_proofs_insert Tree StartIndex IdComms xs_small) =
+  let t := TreeInsertPrep Tree (StartIndex:F) IdComms.head (by
+  apply is_index_in_range_nat_sum (a := StartIndex) (b := b + 1)
+  . simp [D]
+  . rw [<-add_assoc]
+    simp [xs_small])
+  list_of_proofs_insert t (StartIndex+1) IdComms.tail (by
+  simp
+  have : StartIndex + 1 + b = StartIndex + b + 1 := by
+    simp [<-Nat.add_one, add_assoc]
+    simp [add_comm]
+  rw [this]
+  simp [xs_small]) := by
+  simp
+  simp [list_of_items_insert]
+  simp [tree_set_at_fin]
+  simp [TreeInsertPrep]
+  simp [TreeInsert]
+  rw [<-Dir.recover_binary_zmod'_to_dir]
+  . tauto
+  . rw [is_index_in_range_nat] at xs_small
+    rw [ZMod.val_cast_of_lt]
+    . linarith
+    . simp [D] at xs_small
+      simp [Order]
+      linarith
+  . simp [Order, D]
+  . simp [vector_binary_of_bit_to_zmod]
+  . rw [recover_binary_of_to_bits]
+    simp [fin_to_bits_le]
+    split
+    . tauto
+    . contradiction
+
+theorem insertion_loop_equivalence [Fact (perfect_hash poseidon₂)] {b : Nat}
+  (Tree : MerkleTree F poseidon₂ D) (StartIndex : Nat) (IdComms: Vector F b) (xs_small : is_index_in_range_nat D (StartIndex + b)) (hzero : InsertionLoopZero Tree StartIndex IdComms xs_small) (k : F -> Prop) :
+  InsertionLoopTree Tree StartIndex IdComms xs_small (fun newTree => k newTree.root) ↔
+  (let items := list_of_items_insert Tree StartIndex IdComms xs_small
+  let proofs := list_of_proofs_insert Tree StartIndex IdComms xs_small
+  InsertionLoop StartIndex Tree.root items proofs k) := by
+  simp
+  apply Iff.intro
+  . induction b generalizing Tree StartIndex with
     | zero =>
-      simp [InsertionLoop, insertion_circuit]
+      simp [InsertionLoopTree, InsertionLoop]
     | succ _ ih =>
-      simp only [InsertionLoop, insertion_circuit]
-      rintro ⟨hitem, ⟨hproof, ⟨ftree, ⟨hftree, hresult⟩⟩⟩⟩
-      simp [MerkleTree.item_at_nat, Dir.nat_to_dir_vec] at hitem
-      rcases hitem with ⟨bits, ⟨hbits, hitem_at⟩⟩
-      simp [MerkleTree.proof_at_nat, Dir.nat_to_dir_vec] at hproof
-      rcases hproof with ⟨bits', ⟨hbits', hproof_at⟩⟩
-      simp [hbits] at hbits'
-      simp [hbits'] at *
-      simp [MerkleTree.set_at_nat, Dir.nat_to_dir_vec] at hftree
-      rcases hftree with ⟨bits'', ⟨hbits'', hftree_at⟩⟩
-      simp [hbits''] at hbits
-      rw [←Vector.vector_reverse_eq] at hproof_at
-      simp [hbits] at *
-      let t : Vector F D := (Vector.map Bit.toZMod bits')
-      refine ⟨t, ?_⟩
-      refine ⟨?_, ⟨?_, ⟨?_, ?_⟩⟩⟩
-      . apply recover_binary_of_to_bits
-        simp [hbits'']
-      . apply vector_binary_of_bit_to_zmod
-      . simp [<-hproof_at]
-        rw [MerkleTree.recover_tail_equals_recover_reverse, Dir.create_dir_vec_bit, zmod_to_bit_coe, ←hitem_at]
-        simp [MerkleTree.recover_proof_is_root]
-      . rw [MerkleTree.recover_tail_equals_recover_reverse, Dir.create_dir_vec_bit, zmod_to_bit_coe]
-        rw [MerkleTree.proof_insert_invariant (tree := Tree) (old := (0:F)) (new := IdComms.head)]
-        have this : (↑StartIndex + 1:F) = ↑(StartIndex + 1) := by
-          simp [Fin.ext]
+      simp [InsertionLoopZero] at hzero
+      rcases hzero with ⟨hzero', hzero⟩
+      simp only [InsertionLoopTree]
+      rintro ⟨tree, htree, hroot⟩
+      simp only [list_of_items_insert] at htree
+      simp only [Vector.head_cons] at htree
+      rw [insertion_round_prep_uncps] at htree
+      rename_i i _
+      let t₁ := tree
+      let t₂ := TreeInsertPrep Tree (StartIndex) (IdComms.head) (by
+      apply is_index_in_range_nat_sum (a := StartIndex) (b := Nat.succ i)
+      . simp [D]
+      . simp [xs_small])
+      rw [MerkleTree.eq_root_eq_tree (t₁ := t₁) (t₂ := t₂)] at htree
+      simp at htree
+      rw [InsertionLoop]
+      nth_rewrite 1 [list_of_items_insert, list_of_proofs_insert]
+      simp only [Vector.head_cons]
+      rw [insertion_round_prep_uncps]
+      . simp only [list_of_items_insert_tail]
+        simp only [list_of_proofs_insert_tail]
+        rw [htree] at hroot
+        have : @Nat.cast F Semiring.toNatCast StartIndex + 1 = Nat.cast (StartIndex + 1) := by
+          simp [Nat.cast]
         rw [this]
         apply ih
-        linarith only [ixBound]
-        rw [<-hftree_at] at hresult
-        have : ((Nat.cast (Fin.val (Nat.cast StartIndex:F))) + (1:F)) = Nat.cast (StartIndex + 1) := by
-          simp [Nat.cast, NatCast.natCast]
-          simp [Order]
-          rw [<-ZMod.val_nat_cast, ZMod.val_cast_of_lt]
-          simp [Order] at ixBound
-          linarith [ixBound]
-        rw [this] at hresult
-        apply hresult
-        simp [<-hproof_at]
-        simp [<-hitem_at]
-        simp [MerkleTree.recover_proof_is_root]
+        simp [hzero]
+        simp [hroot]
+      . rw [TreeInsertZeroZMod]
+        simp [hzero']
+      . rw [TreeInsertZeroZMod]
+        simp [hzero']
+  . induction b generalizing Tree StartIndex with
+    | zero =>
+      simp [InsertionLoopTree, InsertionLoop]
+    | succ _ ih =>
+      intro htree
+      simp only [InsertionLoopTree]
+      simp [InsertionLoop] at htree
+      rename_i i
+      let t := TreeInsertPrep Tree (StartIndex) (IdComms.head) (by
+        apply is_index_in_range_nat_sum (a := StartIndex) (b := Nat.succ i)
+        . simp [D]
+        . simp [xs_small])
+      refine ⟨t, ?_⟩
+      nth_rewrite 1 [list_of_items_insert, list_of_proofs_insert] at htree
+      simp only [Vector.head_cons] at htree
+      rw [insertion_round_prep_uncps] at htree
+      . rw [insertion_round_prep_uncps, MerkleTree.eq_root_eq_tree]
+        refine ⟨?_, ?_⟩
+        . tauto
+        . apply ih
+          simp [InsertionLoopZero] at hzero
+          rcases hzero with ⟨_, hzero⟩
+          simp [hzero]
+          simp [htree]
+        . rw [TreeInsertZeroZMod]
+          simp [InsertionLoopZero] at hzero
+          rcases hzero with ⟨hzero', _⟩
+          simp [hzero']
+      . apply is_index_in_range_nat_sum (a := StartIndex) (b := Nat.succ i)
+        . simp [D]
+        . simp [xs_small]
+      . rw [TreeInsertZeroZMod]
+        simp [InsertionLoopZero] at hzero
+        rcases hzero with ⟨hzero', _⟩
+        simp [hzero']
+
+theorem insertion_loop_equivalence' [Fact (perfect_hash poseidon₂)] {b : Nat}
+  (Tree : MerkleTree F poseidon₂ D) (StartIndex : Nat) (IdComms: Vector F b) (xs_small : is_index_in_range_nat D (StartIndex + b)) (hzero : InsertionLoopZero Tree StartIndex IdComms xs_small) (k : F -> Prop) :
+  TreeInsertCircuit Tree StartIndex IdComms xs_small (fun newTree => k newTree.root) ↔
+  (let items := list_of_items_insert Tree StartIndex IdComms xs_small
+  let proofs := list_of_proofs_insert Tree StartIndex IdComms xs_small
+  InsertionLoop StartIndex Tree.root items proofs k) := by
+  simp
+  rw [<-insertion_loop_equivalence]
+  apply insertion_loop_uncps
+  . simp [hzero]
+  . simp [hzero]
+
+theorem before_insertion_all_zeroes [Fact (perfect_hash poseidon₂)] {b : Nat}
+  (Tree : MerkleTree F poseidon₂ D) (StartIndex: Nat) (IdComms: Vector F b) (xs_small : is_index_in_range_nat D (StartIndex + b)) :
+  (let items := list_of_items_insert Tree StartIndex IdComms xs_small
+  let proofs := list_of_proofs_insert Tree StartIndex IdComms xs_small
+  InsertionLoop StartIndex Tree.root items proofs k) →
+  InsertionLoopZero Tree StartIndex IdComms xs_small := by
+  simp
+  induction b generalizing Tree StartIndex with
+  | zero => simp [InsertionLoop, InsertionLoopZero]
+  | succ i ih =>
+    intro htree
+    simp [InsertionLoop] at htree
+    simp [InsertionLoopZero]
+    nth_rewrite 1 [list_of_items_insert, list_of_proofs_insert] at htree
+    simp only [Vector.head_cons] at htree
+    rw [insertion_round_prep_uncps] at htree
+    . refine ⟨?_, ?_⟩
+      . apply insertion_round_prep_zero
+        . apply is_index_in_range_nat_sum (a := StartIndex) (b := Nat.succ i)
+          . simp [D]
+          . simp [xs_small]
+        . assumption
+      . apply ih
+        simp [htree]
+    . apply is_index_in_range_nat_sum (a := StartIndex) (b := Nat.succ i)
+      . simp [D]
+      . simp [xs_small]
+    . apply insertion_round_prep_zero
+      . apply is_index_in_range_nat_sum (a := StartIndex) (b := Nat.succ i)
+        . simp [D]
+        . simp [xs_small]
+      . assumption
